Migrated tree code to same as tail call (broken code)

06TreeCode/TreeCodeConversion.thy
@@ -7,17 +7,19 @@ subsection \<open>Compilation to Tree-Code\<close>
 text \<open>This is our first real compilation phase; typechecking and name-removal were fundamentally 
 just modifying an underlying expression, but here we genuinely reshape our expressions into code. 
 The first few steps are simple: encoding an expression means shuffling it into a postfix form, and 
-tree-code closures-values are just encoded stack closure-values.\<close>
+tree-code closures-values are just encoded stack closure-values. We add a \<open>Return\<^sub>e\<close> operation on at 
+the end of ever code block, too; we never encode the \<open>Jump\<^sub>e\<close> operation. Its place will come a little 
+later.\<close>
 
 primrec encode :: "expr\<^sub>d \<Rightarrow> code\<^sub>e list" where
   "encode (Var\<^sub>d x) = [Lookup\<^sub>e x]"
 | "encode (Const\<^sub>d n) = [PushCon\<^sub>e n]"
-| "encode (Lam\<^sub>d t e) = [PushLam\<^sub>e (encode e)]"
+| "encode (Lam\<^sub>d t e) = [PushLam\<^sub>e (encode e) Return\<^sub>e]"
 | "encode (App\<^sub>d e\<^sub>1 e\<^sub>2) = encode e\<^sub>1 @ encode e\<^sub>2 @ [Apply\<^sub>e]"
 
 primrec encode_closure :: "closure\<^sub>c \<Rightarrow> closure\<^sub>e" where
   "encode_closure (Const\<^sub>c n) = Const\<^sub>e n"
-| "encode_closure (Lam\<^sub>c t \<Delta> e) = Lam\<^sub>e (map encode_closure \<Delta>) (encode e)"
+| "encode_closure (Lam\<^sub>c t \<Delta> e) = Lam\<^sub>e (map encode_closure \<Delta>) (encode e) Return\<^sub>e"
 
 lemma tl_encode [simp]: "tl (encode e @ \<C>) = tl (encode e) @ \<C>"
   by (induction e arbitrary: \<C>) simp_all
@@ -41,14 +43,14 @@ what environment) callstack frames begin.\<close>
 
 fun prepend_to_top_frame :: "code\<^sub>e list \<Rightarrow> frame\<^sub>e list \<Rightarrow> frame\<^sub>e list" where
   "prepend_to_top_frame \<C> [] = []"
-| "prepend_to_top_frame \<C> ((\<Delta>, \<C>') # s\<^sub>e) = (\<Delta>, \<C> @ \<C>') # s\<^sub>e"
+| "prepend_to_top_frame \<C> ((\<Delta>, \<C>', r) # s\<^sub>e) = (\<Delta>, \<C> @ \<C>', r) # s\<^sub>e"
 
 fun stack_from_stack :: "frame\<^sub>c list \<Rightarrow> frame\<^sub>e list" where
   "stack_from_stack [] = []"
 | "stack_from_stack (FApp1\<^sub>c \<Delta>' e # s\<^sub>c) = 
     prepend_to_top_frame (encode e @ [Apply\<^sub>e]) (stack_from_stack s\<^sub>c)"
 | "stack_from_stack (FApp2\<^sub>c c # s\<^sub>c) = prepend_to_top_frame [Apply\<^sub>e] (stack_from_stack s\<^sub>c)"
-| "stack_from_stack (FReturn\<^sub>c \<Delta> # s\<^sub>c) = (map encode_closure \<Delta>, []) # stack_from_stack s\<^sub>c"
+| "stack_from_stack (FReturn\<^sub>c \<Delta> # s\<^sub>c) = (map encode_closure \<Delta>, [], Return\<^sub>e) # stack_from_stack s\<^sub>c"
 
 lemma prepend_nil [simp]: "prepend_to_top_frame [] s\<^sub>e = s\<^sub>e"
   by (induction "[] :: code\<^sub>e list" s\<^sub>e rule: prepend_to_top_frame.induct) simp_all
@@ -72,7 +74,7 @@ We again have to use \<open>iter\<close> in our statement of the theorem, becaus
 steps (\<open>ret\<^sub>c_app1\<close> and \<open>ret\<^sub>c_app2\<close>) are not matched by any steps in the tree-code evaluation.\<close>
 
 lemma lookup_latest [dest]: "latest_environment s\<^sub>c = Some \<Delta> \<Longrightarrow> 
-    \<exists>\<C> s\<^sub>e. stack_from_stack s\<^sub>c = (map encode_closure \<Delta>, \<C>) # s\<^sub>e"
+    \<exists>\<C> s\<^sub>e. stack_from_stack s\<^sub>c = (map encode_closure \<Delta>, \<C>, Return\<^sub>e) # s\<^sub>e"
   by (induction s\<^sub>c rule: stack_from_stack.induct) auto
 
 theorem correct\<^sub>e [simp]: "\<Sigma> \<leadsto>\<^sub>c \<Sigma>' \<Longrightarrow> \<Sigma> :\<^sub>c t \<Longrightarrow> iter (\<leadsto>\<^sub>e) (encode_state \<Sigma>) (encode_state \<Sigma>')"
@@ -80,64 +82,61 @@ proof (induction \<Sigma> \<Sigma>' rule: eval\<^sub>c.induct)
   case (ev\<^sub>c_var \<Delta> x c s\<^sub>c)
   then obtain t' \<Gamma> where "(s\<^sub>c :\<^sub>c t' \<rightarrow> t) \<and> (\<Delta> :\<^sub>c\<^sub>l\<^sub>s \<Gamma>) \<and> latest_environment s\<^sub>c = Some \<Delta> \<and> 
     lookup \<Gamma> x = Some t'" by fastforce
-  then obtain \<C> s\<^sub>e where S: "stack_from_stack s\<^sub>c = (map encode_closure \<Delta>, \<C>) # s\<^sub>e" 
-    by auto
-  with ev\<^sub>c_var have "S\<^sub>e (vals_from_stack s\<^sub>c) ((map encode_closure \<Delta>, Lookup\<^sub>e x # \<C>) # s\<^sub>e) \<leadsto>\<^sub>e 
-    S\<^sub>e (encode_closure c # vals_from_stack s\<^sub>c) ((map encode_closure \<Delta>, \<C>) # s\<^sub>e)" by simp
-  hence "iter (\<leadsto>\<^sub>e) (S\<^sub>e (vals_from_stack s\<^sub>c) ((map encode_closure \<Delta>, Lookup\<^sub>e x # \<C>) # s\<^sub>e))
-    (S\<^sub>e (encode_closure c # vals_from_stack s\<^sub>c) ((map encode_closure \<Delta>, \<C>) # s\<^sub>e))" 
+  then obtain \<C> s\<^sub>e where S: "stack_from_stack s\<^sub>c = (map encode_closure \<Delta>, \<C>, Return\<^sub>e) # s\<^sub>e" by auto
+  with ev\<^sub>c_var have "S\<^sub>e (vals_from_stack s\<^sub>c) ((map encode_closure \<Delta>, Lookup\<^sub>e x # \<C>, Return\<^sub>e) # s\<^sub>e) \<leadsto>\<^sub>e 
+    S\<^sub>e (encode_closure c # vals_from_stack s\<^sub>c) ((map encode_closure \<Delta>, \<C>, Return\<^sub>e) # s\<^sub>e)" by simp
+  hence "iter (\<leadsto>\<^sub>e) (S\<^sub>e (vals_from_stack s\<^sub>c) ((map encode_closure \<Delta>, Lookup\<^sub>e x # \<C>, Return\<^sub>e) # s\<^sub>e))
+    (S\<^sub>e (encode_closure c # vals_from_stack s\<^sub>c) ((map encode_closure \<Delta>, \<C>, Return\<^sub>e) # s\<^sub>e))" 
       by (metis iter_one)
-    with S show ?case by simp
+  with S show ?case by simp
 next
   case (ev\<^sub>c_con s\<^sub>c \<Delta> n)
-  then obtain \<Gamma> where "(s\<^sub>c :\<^sub>c Num \<rightarrow> t) \<and> (\<Delta> :\<^sub>c\<^sub>l\<^sub>s \<Gamma>) \<and> latest_environment s\<^sub>c = Some \<Delta>" 
-    by fastforce
-  then obtain \<C> s\<^sub>e where S: "stack_from_stack s\<^sub>c = (map encode_closure \<Delta>, \<C>) # s\<^sub>e" 
-    by auto
-  have "S\<^sub>e (vals_from_stack s\<^sub>c) ((map encode_closure \<Delta>, PushCon\<^sub>e n # \<C>) # s\<^sub>e) \<leadsto>\<^sub>e 
-    S\<^sub>e (Const\<^sub>e n # vals_from_stack s\<^sub>c) ((map encode_closure \<Delta>, \<C>) # s\<^sub>e)" by simp
-  hence "iter (\<leadsto>\<^sub>e) (S\<^sub>e (vals_from_stack s\<^sub>c) ((map encode_closure \<Delta>, PushCon\<^sub>e n # \<C>) # s\<^sub>e)) 
-    (S\<^sub>e (Const\<^sub>e n # vals_from_stack s\<^sub>c) ((map encode_closure \<Delta>, \<C>) # s\<^sub>e))" by (metis iter_one)
+  then obtain \<Gamma> where "(s\<^sub>c :\<^sub>c Num \<rightarrow> t) \<and> (\<Delta> :\<^sub>c\<^sub>l\<^sub>s \<Gamma>) \<and> latest_environment s\<^sub>c = Some \<Delta>" by fastforce
+  then obtain \<C> s\<^sub>e where S: "stack_from_stack s\<^sub>c = (map encode_closure \<Delta>, \<C>, Return\<^sub>e) # s\<^sub>e" by auto
+  have "S\<^sub>e (vals_from_stack s\<^sub>c) ((map encode_closure \<Delta>, PushCon\<^sub>e n # \<C>, Return\<^sub>e) # s\<^sub>e) \<leadsto>\<^sub>e 
+    S\<^sub>e (Const\<^sub>e n # vals_from_stack s\<^sub>c) ((map encode_closure \<Delta>, \<C>, Return\<^sub>e) # s\<^sub>e)" by simp
+  hence "iter (\<leadsto>\<^sub>e) (S\<^sub>e (vals_from_stack s\<^sub>c) ((map encode_closure \<Delta>, PushCon\<^sub>e n # \<C>, Return\<^sub>e) # s\<^sub>e)) 
+    (S\<^sub>e (Const\<^sub>e n # vals_from_stack s\<^sub>c) ((map encode_closure \<Delta>, \<C>, Return\<^sub>e) # s\<^sub>e))" 
+      by (metis iter_one)
   with S show ?case by simp
 next
   case (ev\<^sub>c_lam s\<^sub>c \<Delta> tt e)
   then obtain t' \<Gamma> where "(s\<^sub>c :\<^sub>c t' \<rightarrow> t) \<and> (\<Delta> :\<^sub>c\<^sub>l\<^sub>s \<Gamma>) \<and> latest_environment s\<^sub>c = Some \<Delta> \<and>
     (\<Gamma> \<turnstile>\<^sub>d Lam\<^sub>d tt e : t')" by fastforce
-  then obtain \<C> s\<^sub>e where S: "stack_from_stack s\<^sub>c = (map encode_closure \<Delta>, \<C>) # s\<^sub>e" 
-    by auto
-  hence "S\<^sub>e (vals_from_stack s\<^sub>c) ((map encode_closure \<Delta>, PushLam\<^sub>e (encode e) # \<C>) # s\<^sub>e) \<leadsto>\<^sub>e 
-    S\<^sub>e (Lam\<^sub>e (map encode_closure \<Delta>) (encode e) # vals_from_stack s\<^sub>c) 
-      ((map encode_closure \<Delta>, \<C>) # s\<^sub>e)" by (metis ev\<^sub>e_pushlam)
+  then obtain \<C> s\<^sub>e where S: "stack_from_stack s\<^sub>c = (map encode_closure \<Delta>, \<C>, Return\<^sub>e) # s\<^sub>e" by auto
+  hence "S\<^sub>e (vals_from_stack s\<^sub>c) 
+    ((map encode_closure \<Delta>, PushLam\<^sub>e (encode e) Return\<^sub>e # \<C>, Return\<^sub>e) # s\<^sub>e) \<leadsto>\<^sub>e 
+    S\<^sub>e (Lam\<^sub>e (map encode_closure \<Delta>) (encode e) Return\<^sub>e # vals_from_stack s\<^sub>c) 
+    ((map encode_closure \<Delta>, \<C>, Return\<^sub>e) # s\<^sub>e)" by (metis ev\<^sub>e_pushlam)
   hence "iter (\<leadsto>\<^sub>e) (S\<^sub>e (vals_from_stack s\<^sub>c) 
-    ((map encode_closure \<Delta>, PushLam\<^sub>e (encode e) # \<C>) # s\<^sub>e)) 
-      (S\<^sub>e (Lam\<^sub>e (map encode_closure \<Delta>) (encode e) # vals_from_stack s\<^sub>c)
-        ((map encode_closure \<Delta>, \<C>) # s\<^sub>e))" by (metis iter_one)
+    ((map encode_closure \<Delta>, PushLam\<^sub>e (encode e) Return\<^sub>e # \<C>, Return\<^sub>e) # s\<^sub>e)) 
+    (S\<^sub>e (Lam\<^sub>e (map encode_closure \<Delta>) (encode e) Return\<^sub>e # vals_from_stack s\<^sub>c)
+    ((map encode_closure \<Delta>, \<C>, Return\<^sub>e) # s\<^sub>e))" by (metis iter_one)
   with S show ?case by (simp add: encode_def)
 next
   case (ret\<^sub>c_app2 t\<^sub>1 \<Delta> e\<^sub>1 s\<^sub>c c\<^sub>2)
   then obtain \<Gamma> t\<^sub>2 \<Delta>' where "(\<Delta> :\<^sub>c\<^sub>l\<^sub>s \<Gamma>) \<and> (insert_at 0 t\<^sub>1 \<Gamma> \<turnstile>\<^sub>d e\<^sub>1 : t\<^sub>2) \<and> (s\<^sub>c :\<^sub>c t\<^sub>2 \<rightarrow> t) \<and> 
     latest_environment s\<^sub>c = Some \<Delta>' \<and> (c\<^sub>2 :\<^sub>c\<^sub>l t\<^sub>1)" by blast
-  then obtain \<C> s\<^sub>e where S: "stack_from_stack s\<^sub>c = (map encode_closure \<Delta>', \<C>) # s\<^sub>e" 
-    by auto
-  hence "S\<^sub>e (encode_closure c\<^sub>2 # Lam\<^sub>e (map encode_closure \<Delta>) (encode e\<^sub>1) # 
-    vals_from_stack s\<^sub>c) ((map encode_closure \<Delta>', Apply\<^sub>e # \<C>) # s\<^sub>e) \<leadsto>\<^sub>e
-      S\<^sub>e (vals_from_stack s\<^sub>c) ((encode_closure c\<^sub>2 # map encode_closure \<Delta>, 
-        encode e\<^sub>1) # stack_from_stack s\<^sub>c)" by (metis ev\<^sub>e_apply)
+  then obtain \<C> s\<^sub>e where S: "stack_from_stack s\<^sub>c = (map encode_closure \<Delta>', \<C>, Return\<^sub>e) # s\<^sub>e" by auto
+  hence "S\<^sub>e (encode_closure c\<^sub>2 # Lam\<^sub>e (map encode_closure \<Delta>) (encode e\<^sub>1) Return\<^sub>e # 
+    vals_from_stack s\<^sub>c) ((map encode_closure \<Delta>', Apply\<^sub>e # \<C>, Return\<^sub>e) # s\<^sub>e) \<leadsto>\<^sub>e
+    S\<^sub>e (vals_from_stack s\<^sub>c) ((encode_closure c\<^sub>2 # map encode_closure \<Delta>, encode e\<^sub>1, Return\<^sub>e) # 
+    stack_from_stack s\<^sub>c)" by (metis ev\<^sub>e_apply)
   hence "iter (\<leadsto>\<^sub>e)
-    (S\<^sub>e (encode_closure c\<^sub>2 # Lam\<^sub>e (map encode_closure \<Delta>) (encode e\<^sub>1) # 
-      vals_from_stack s\<^sub>c) ((map encode_closure \<Delta>', Apply\<^sub>e # \<C>) # s\<^sub>e))
-        (S\<^sub>e (vals_from_stack s\<^sub>c) ((encode_closure c\<^sub>2 # map encode_closure \<Delta>, 
-          encode e\<^sub>1) # stack_from_stack s\<^sub>c))"
-    by (metis iter_one)
+    (S\<^sub>e (encode_closure c\<^sub>2 # Lam\<^sub>e (map encode_closure \<Delta>) (encode e\<^sub>1) Return\<^sub>e # vals_from_stack s\<^sub>c) 
+    ((map encode_closure \<Delta>', Apply\<^sub>e # \<C>, Return\<^sub>e) # s\<^sub>e)) 
+    (S\<^sub>e (vals_from_stack s\<^sub>c) ((encode_closure c\<^sub>2 # map encode_closure \<Delta>, encode e\<^sub>1, Return\<^sub>e) # 
+    stack_from_stack s\<^sub>c))" by (metis iter_one)
   with S show ?case by (simp add: encode_def)
 next
   case (ret\<^sub>c_ret \<Delta> s\<^sub>c c)
-  have "S\<^sub>e (encode_closure c # vals_from_stack s\<^sub>c) 
-    ((map encode_closure \<Delta>, []) # stack_from_stack s\<^sub>c) \<leadsto>\<^sub>e
-      S\<^sub>e (encode_closure c # vals_from_stack s\<^sub>c) (stack_from_stack s\<^sub>c)" by simp
+  have "S\<^sub>e (encode_closure c # vals_from_stack s\<^sub>c) ((map encode_closure \<Delta>, [], Return\<^sub>e) # 
+    stack_from_stack s\<^sub>c) \<leadsto>\<^sub>e
+    S\<^sub>e (encode_closure c # vals_from_stack s\<^sub>c) (stack_from_stack s\<^sub>c)" by simp
   hence "iter (\<leadsto>\<^sub>e) 
-    (S\<^sub>e (encode_closure c # vals_from_stack s\<^sub>c) ((map encode_closure \<Delta>, []) # stack_from_stack s\<^sub>c))
-      (S\<^sub>e (encode_closure c # vals_from_stack s\<^sub>c) (stack_from_stack s\<^sub>c))" by (metis iter_one)
+    (S\<^sub>e (encode_closure c # vals_from_stack s\<^sub>c) ((map encode_closure \<Delta>, [], Return\<^sub>e) # 
+    stack_from_stack s\<^sub>c))
+    (S\<^sub>e (encode_closure c # vals_from_stack s\<^sub>c) (stack_from_stack s\<^sub>c))" by (metis iter_one)
   thus ?case by simp
 qed fastforce+
 
@@ -198,120 +197,128 @@ lemma encode_to_pushcon [dest]: "encode e @ \<C>' = PushCon\<^sub>e n # \<C> \<L
     head_expr e = Const\<^sub>d n \<and> \<C> = tl (encode e) @ \<C>'"
   by (induction e arbitrary: \<C>') fastforce+
 
-lemma encode_to_pushlam [dest]: "encode e @ \<C>' = PushLam\<^sub>e \<C>'' # \<C> \<Longrightarrow> 
-    \<exists>t e'. head_expr e = Lam\<^sub>d t e' \<and> \<C>'' = encode e' \<and> \<C> = tl (encode e) @ \<C>'"
+lemma encode_to_pushlam [dest]: "encode e @ \<C>' = PushLam\<^sub>e \<C>'' r # \<C> \<Longrightarrow> 
+    \<exists>t e'. head_expr e = Lam\<^sub>d t e' \<and> \<C>'' = encode e' \<and> \<C> = tl (encode e) @ \<C>' \<and> r = Return\<^sub>e"
   by (induction e arbitrary: \<C>') fastforce+
 
 lemma encode_to_apply [dest]: "encode e @ \<C>' = Apply\<^sub>e # \<C> \<Longrightarrow> False"
   by (induction e arbitrary: \<C>') simp_all
 
-lemma encode_lam_closure [dest]: "Lam\<^sub>e env \<C> = encode_closure c \<Longrightarrow> 
-    \<exists>t \<Delta> e. c = Lam\<^sub>c t \<Delta> e \<and> env = map encode_closure \<Delta> \<and> \<C> = encode e"
+lemma encode_lam_closure [dest]: "Lam\<^sub>e env \<C> r = encode_closure c \<Longrightarrow> 
+    \<exists>t \<Delta> e. c = Lam\<^sub>c t \<Delta> e \<and> env = map encode_closure \<Delta> \<and> \<C> = encode e \<and> r = Return\<^sub>e"
   by (induction c) simp_all
 
-lemma prepend_to_cons [dest]: "prepend_to_top_frame \<C>' s\<^sub>e = (\<Delta>, \<C>) # s\<^sub>e' \<Longrightarrow> 
-    \<exists>\<C>''. s\<^sub>e = (\<Delta>, \<C>'') # s\<^sub>e' \<and> \<C> = \<C>' @ \<C>''"
+lemma prepend_to_cons [dest]: "prepend_to_top_frame \<C>' s\<^sub>e = (\<Delta>, \<C>, r) # s\<^sub>e' \<Longrightarrow> 
+    \<exists>\<C>''. s\<^sub>e = (\<Delta>, \<C>'', r) # s\<^sub>e' \<and> \<C> = \<C>' @ \<C>''"
   by (induction \<C>' s\<^sub>e rule: prepend_to_top_frame.induct) simp_all
 
-lemma prepend_to_apply [dest]: "prepend_to_top_frame (encode e) s\<^sub>e = (\<Delta>, Apply\<^sub>e # \<C>) # s\<^sub>e' \<Longrightarrow> 
+lemma prepend_to_apply [dest]: "prepend_to_top_frame (encode e) s\<^sub>e = (\<Delta>, Apply\<^sub>e # \<C>, r) # s\<^sub>e' \<Longrightarrow> 
     False"
   by (induction "encode e" s\<^sub>e rule: prepend_to_top_frame.induct) auto
 
-lemma encode_stack_to_lookup [dest]: "stack_from_stack s\<^sub>c = (\<Delta>\<^sub>e, Lookup\<^sub>e x # \<C>) # s\<^sub>e \<Longrightarrow> 
-  \<exists>\<Delta>\<^sub>c e s\<^sub>c' \<C>'. s\<^sub>c = FApp1\<^sub>c \<Delta>\<^sub>c e # s\<^sub>c' \<and> stack_from_stack s\<^sub>c' = (\<Delta>\<^sub>e, \<C>') # s\<^sub>e \<and> 
+lemma encode_stack_to_lookup [dest]: "stack_from_stack s\<^sub>c = (\<Delta>\<^sub>e, Lookup\<^sub>e x # \<C>, r) # s\<^sub>e \<Longrightarrow> 
+  \<exists>\<Delta>\<^sub>c e s\<^sub>c' \<C>'. s\<^sub>c = FApp1\<^sub>c \<Delta>\<^sub>c e # s\<^sub>c' \<and> stack_from_stack s\<^sub>c' = (\<Delta>\<^sub>e, \<C>', r) # s\<^sub>e \<and> 
     head_expr e = Var\<^sub>d x \<and> \<C> = tl (encode e) @ Apply\<^sub>e # \<C>'"
 proof (induction s\<^sub>c rule: stack_from_stack.induct)
   case (2 \<Delta> e s\<^sub>c)
-  then obtain \<C>' where "stack_from_stack s\<^sub>c = (\<Delta>\<^sub>e, \<C>') # s\<^sub>e \<and> 
+  then obtain \<C>' where "stack_from_stack s\<^sub>c = (\<Delta>\<^sub>e, \<C>', r) # s\<^sub>e \<and> 
     encode e @ Apply\<^sub>e # \<C>' = Lookup\<^sub>e x # \<C>" by fastforce
   thus ?case by auto
 qed auto
 
-lemma encode_stack_to_pushcon [dest]: "stack_from_stack s\<^sub>c = (\<Delta>\<^sub>e, PushCon\<^sub>e n # \<C>) # s\<^sub>e \<Longrightarrow> 
-  \<exists>\<Delta>\<^sub>c e s\<^sub>c' \<C>'. s\<^sub>c = FApp1\<^sub>c \<Delta>\<^sub>c e # s\<^sub>c' \<and> stack_from_stack s\<^sub>c' = (\<Delta>\<^sub>e, \<C>') # s\<^sub>e \<and> 
+lemma encode_stack_to_pushcon [dest]: "stack_from_stack s\<^sub>c = (\<Delta>\<^sub>e, PushCon\<^sub>e n # \<C>, r) # s\<^sub>e \<Longrightarrow> 
+  \<exists>\<Delta>\<^sub>c e s\<^sub>c' \<C>'. s\<^sub>c = FApp1\<^sub>c \<Delta>\<^sub>c e # s\<^sub>c' \<and> stack_from_stack s\<^sub>c' = (\<Delta>\<^sub>e, \<C>', r) # s\<^sub>e \<and> 
     head_expr e = Const\<^sub>d n \<and> \<C> = tl (encode e) @ Apply\<^sub>e # \<C>'"
 proof (induction s\<^sub>c rule: stack_from_stack.induct)
   case (2 \<Delta>\<^sub>s e s\<^sub>c)
-  then obtain \<C>' where "stack_from_stack s\<^sub>c = (\<Delta>\<^sub>e, \<C>') # s\<^sub>e \<and> 
+  then obtain \<C>' where "stack_from_stack s\<^sub>c = (\<Delta>\<^sub>e, \<C>', r) # s\<^sub>e \<and> 
     encode e @ Apply\<^sub>e # \<C>' = PushCon\<^sub>e n # \<C>" by fastforce
   thus ?case by auto
 qed auto
 
-lemma encode_stack_to_pushlam [dest]: "stack_from_stack s\<^sub>c = (\<Delta>\<^sub>e, PushLam\<^sub>e \<C>' # \<C>) # s\<^sub>e \<Longrightarrow> 
-  \<exists>\<Delta>\<^sub>c e s\<^sub>c' t e' \<C>''. s\<^sub>c = FApp1\<^sub>c \<Delta>\<^sub>c e # s\<^sub>c' \<and> stack_from_stack s\<^sub>c' = (\<Delta>\<^sub>e, \<C>'') # s\<^sub>e \<and> 
-    head_expr e = Lam\<^sub>d t e' \<and> \<C> = tl (encode e) @ Apply\<^sub>e # \<C>'' \<and> \<C>' = encode e'"
+lemma encode_stack_to_pushlam [dest]: "stack_from_stack s\<^sub>c = (\<Delta>\<^sub>e, PushLam\<^sub>e \<C>' r' # \<C>, r) # s\<^sub>e \<Longrightarrow> 
+  \<exists>\<Delta>\<^sub>c e s\<^sub>c' t e' \<C>''. s\<^sub>c = FApp1\<^sub>c \<Delta>\<^sub>c e # s\<^sub>c' \<and> stack_from_stack s\<^sub>c' = (\<Delta>\<^sub>e, \<C>'', r) # s\<^sub>e \<and> 
+    head_expr e = Lam\<^sub>d t e' \<and> \<C> = tl (encode e) @ Apply\<^sub>e # \<C>'' \<and> \<C>' = encode e' \<and> r' = Return\<^sub>e"
 proof (induction s\<^sub>c rule: stack_from_stack.induct)
   case (2 \<Delta>\<^sub>c e s\<^sub>c)
-  then obtain \<C>'' where "stack_from_stack s\<^sub>c = (\<Delta>\<^sub>e, \<C>'') # s\<^sub>e \<and> 
-    encode e @ Apply\<^sub>e # \<C>'' = PushLam\<^sub>e \<C>' # \<C>" by fastforce
+  then obtain \<C>'' where "stack_from_stack s\<^sub>c = (\<Delta>\<^sub>e, \<C>'', r) # s\<^sub>e \<and> 
+    encode e @ Apply\<^sub>e # \<C>'' = PushLam\<^sub>e \<C>' r' # \<C>" by fastforce
   moreover then obtain t e' where "head_expr e = Lam\<^sub>d t e' \<and> \<C>' = encode e' \<and> 
-    \<C> = tl (encode e) @ Apply\<^sub>e # \<C>''" by (metis encode_to_pushlam)
-  ultimately show ?case by fastforce
+    \<C> = tl (encode e) @ Apply\<^sub>e # \<C>'' \<and> r' = Return\<^sub>e" by (metis encode_to_pushlam)
+  ultimately show ?case by auto
 qed auto
 
-lemma encode_stack_to_apply [dest]: "stack_from_stack s = (\<Delta>\<^sub>e, Apply\<^sub>e # \<C>) # s\<^sub>e \<Longrightarrow> 
-    \<exists>s\<^sub>c' c. s = FApp2\<^sub>c c # s\<^sub>c' \<and> stack_from_stack s\<^sub>c' = (\<Delta>\<^sub>e, \<C>) # s\<^sub>e"
-  by (induction s rule: stack_from_stack.induct) auto
+lemma encode_stack_to_apply [dest]: "stack_from_stack s = (\<Delta>\<^sub>e, Apply\<^sub>e # \<C>, r) # s\<^sub>e \<Longrightarrow> 
+    \<exists>s\<^sub>c' c. s = FApp2\<^sub>c c # s\<^sub>c' \<and> stack_from_stack s\<^sub>c' = (\<Delta>\<^sub>e, \<C>, r) # s\<^sub>e"
+proof (induction s rule: stack_from_stack.induct)
+  case (3 c s\<^sub>c)
+  then show ?case by auto
+qed auto
 
-lemma encode_stack_to_return [dest]: "stack_from_stack s = (\<Delta>\<^sub>e, []) # s\<^sub>e \<Longrightarrow> 
-    \<exists>\<Delta>\<^sub>c s\<^sub>c'. s = FReturn\<^sub>c \<Delta>\<^sub>c # s\<^sub>c' \<and> \<Delta>\<^sub>e = map encode_closure \<Delta>\<^sub>c \<and> s\<^sub>e = stack_from_stack s\<^sub>c'"
+lemma encode_stack_to_return [dest]: "stack_from_stack s = (\<Delta>\<^sub>e, [], r) # s\<^sub>e \<Longrightarrow> 
+  \<exists>\<Delta>\<^sub>c s\<^sub>c'. s = FReturn\<^sub>c \<Delta>\<^sub>c # s\<^sub>c' \<and> \<Delta>\<^sub>e = map encode_closure \<Delta>\<^sub>c \<and> s\<^sub>e = stack_from_stack s\<^sub>c' \<and> 
+    r = Return\<^sub>e"
   by (induction s rule: stack_from_stack.induct) auto
 
 lemma encode_state_to_lookup [dest, consumes 1, case_names SE\<^sub>c SC\<^sub>c]: "
-  encode_state \<Sigma>\<^sub>c = S\<^sub>e \<V> ((\<Delta>\<^sub>e, Lookup\<^sub>e x # \<C>) # s\<^sub>e) \<Longrightarrow> 
+  encode_state \<Sigma>\<^sub>c = S\<^sub>e \<V> ((\<Delta>\<^sub>e, Lookup\<^sub>e x # \<C>, r) # s\<^sub>e) \<Longrightarrow> 
     (\<And>s\<^sub>c \<Delta>\<^sub>c e \<C>'. head_expr e = Var\<^sub>d x \<Longrightarrow> \<C> = tl (encode e) @ \<C>' \<Longrightarrow> 
-      stack_from_stack s\<^sub>c = ((\<Delta>\<^sub>e, \<C>') # s\<^sub>e) \<Longrightarrow> \<V> = vals_from_stack s\<^sub>c \<Longrightarrow> P (SE\<^sub>c s\<^sub>c \<Delta>\<^sub>c e)) \<Longrightarrow> 
+      stack_from_stack s\<^sub>c = ((\<Delta>\<^sub>e, \<C>', r) # s\<^sub>e) \<Longrightarrow> \<V> = vals_from_stack s\<^sub>c \<Longrightarrow> P (SE\<^sub>c s\<^sub>c \<Delta>\<^sub>c e)) \<Longrightarrow> 
     (\<And>s\<^sub>c c \<Delta>\<^sub>c e \<C>'. head_expr e = Var\<^sub>d x \<Longrightarrow> \<C> = tl (encode e) @ Apply\<^sub>e # \<C>' \<Longrightarrow> 
-      stack_from_stack s\<^sub>c = ((\<Delta>\<^sub>e, \<C>') # s\<^sub>e) \<Longrightarrow> \<V> = encode_closure c # vals_from_stack s\<^sub>c \<Longrightarrow> 
+      stack_from_stack s\<^sub>c = ((\<Delta>\<^sub>e, \<C>', r) # s\<^sub>e) \<Longrightarrow> \<V> = encode_closure c # vals_from_stack s\<^sub>c \<Longrightarrow> 
       P (SC\<^sub>c (FApp1\<^sub>c \<Delta>\<^sub>c e # s\<^sub>c) c)) \<Longrightarrow> P \<Sigma>\<^sub>c"
 proof (induction \<Sigma>\<^sub>c)
   case (SE\<^sub>c s \<Delta> e)
-  moreover then obtain \<C>' where "stack_from_stack s = (\<Delta>\<^sub>e, \<C>') # s\<^sub>e \<and> 
+  moreover then obtain \<C>' where "stack_from_stack s = (\<Delta>\<^sub>e, \<C>', r) # s\<^sub>e \<and> 
     encode e @ \<C>' = Lookup\<^sub>e x # \<C>" by auto
   ultimately show ?case by auto
 qed auto
 
 lemma encode_state_to_pushcon [dest, consumes 1, case_names SE\<^sub>c SC\<^sub>c]: "
-  encode_state \<Sigma>\<^sub>c = S\<^sub>e \<V> ((\<Delta>\<^sub>e, PushCon\<^sub>e n # \<C>) # s\<^sub>e) \<Longrightarrow> 
+  encode_state \<Sigma>\<^sub>c = S\<^sub>e \<V> ((\<Delta>\<^sub>e, PushCon\<^sub>e n # \<C>, r) # s\<^sub>e) \<Longrightarrow> 
     (\<And>s\<^sub>c \<Delta>\<^sub>c e \<C>'. head_expr e = Const\<^sub>d n \<Longrightarrow> \<C> = tl (encode e) @ \<C>' \<Longrightarrow> 
-      stack_from_stack s\<^sub>c = ((\<Delta>\<^sub>e, \<C>') # s\<^sub>e) \<Longrightarrow> \<V> = vals_from_stack s\<^sub>c \<Longrightarrow> P (SE\<^sub>c s\<^sub>c \<Delta>\<^sub>c e)) \<Longrightarrow> 
+      stack_from_stack s\<^sub>c = ((\<Delta>\<^sub>e, \<C>', r) # s\<^sub>e) \<Longrightarrow> \<V> = vals_from_stack s\<^sub>c \<Longrightarrow> P (SE\<^sub>c s\<^sub>c \<Delta>\<^sub>c e)) \<Longrightarrow> 
     (\<And>s\<^sub>c c \<Delta>\<^sub>c e \<C>'. head_expr e = Const\<^sub>d n \<Longrightarrow> \<C> = tl (encode e) @ Apply\<^sub>e # \<C>' \<Longrightarrow> 
-      stack_from_stack s\<^sub>c = ((\<Delta>\<^sub>e, \<C>') # s\<^sub>e) \<Longrightarrow> \<V> = encode_closure c # vals_from_stack s\<^sub>c \<Longrightarrow> 
+      stack_from_stack s\<^sub>c = ((\<Delta>\<^sub>e, \<C>', r) # s\<^sub>e) \<Longrightarrow> \<V> = encode_closure c # vals_from_stack s\<^sub>c \<Longrightarrow> 
       P (SC\<^sub>c (FApp1\<^sub>c \<Delta>\<^sub>c e # s\<^sub>c) c)) \<Longrightarrow> P \<Sigma>\<^sub>c"
 proof (induction \<Sigma>\<^sub>c)
   case (SE\<^sub>c s \<Delta> e)
-  moreover then obtain \<C>' where "stack_from_stack s = (\<Delta>\<^sub>e, \<C>') # s\<^sub>e \<and> 
+  moreover then obtain \<C>' where "stack_from_stack s = (\<Delta>\<^sub>e, \<C>', r) # s\<^sub>e \<and> 
     encode e @ \<C>' = PushCon\<^sub>e n # \<C>" by auto
   ultimately show ?case by auto
 qed auto
 
 lemma encode_state_to_pushlam [dest, consumes 1, case_names SE\<^sub>c SC\<^sub>c]: "
-  encode_state \<Sigma>\<^sub>c = S\<^sub>e \<V> ((\<Delta>\<^sub>e, PushLam\<^sub>e \<C>' # \<C>) # s\<^sub>e) \<Longrightarrow> 
+  encode_state \<Sigma>\<^sub>c = S\<^sub>e \<V> ((\<Delta>\<^sub>e, PushLam\<^sub>e \<C>' r' # \<C>, r) # s\<^sub>e) \<Longrightarrow> 
     (\<And>s\<^sub>c \<Delta>\<^sub>c e tt e' \<C>''. \<Sigma>\<^sub>c = SE\<^sub>c s\<^sub>c \<Delta>\<^sub>c e \<Longrightarrow> head_expr e = Lam\<^sub>d tt e' \<Longrightarrow> 
       \<C> = tl (encode e) @ \<C>'' \<Longrightarrow> \<C>' = encode e' \<Longrightarrow> \<V> = vals_from_stack s\<^sub>c \<Longrightarrow> 
-      stack_from_stack s\<^sub>c = (\<Delta>\<^sub>e, \<C>'') # s\<^sub>e \<Longrightarrow> P) \<Longrightarrow> 
+      stack_from_stack s\<^sub>c = (\<Delta>\<^sub>e, \<C>'', r) # s\<^sub>e \<Longrightarrow> r' = Return\<^sub>e \<Longrightarrow> P) \<Longrightarrow> 
     (\<And>s\<^sub>c c \<Delta>\<^sub>c e tt e' \<C>''. \<Sigma>\<^sub>c = SC\<^sub>c (FApp1\<^sub>c \<Delta>\<^sub>c e # s\<^sub>c) c \<Longrightarrow> head_expr e = Lam\<^sub>d tt e' \<Longrightarrow> 
       \<C> = tl (encode e) @ Apply\<^sub>e # \<C>'' \<Longrightarrow> \<C>' = encode e' \<Longrightarrow> 
-      \<V> = encode_closure c # vals_from_stack s\<^sub>c \<Longrightarrow> stack_from_stack s\<^sub>c = (\<Delta>\<^sub>e, \<C>'') # s\<^sub>e \<Longrightarrow> P) \<Longrightarrow> 
+      \<V> = encode_closure c # vals_from_stack s\<^sub>c \<Longrightarrow> stack_from_stack s\<^sub>c = (\<Delta>\<^sub>e, \<C>'', r) # s\<^sub>e \<Longrightarrow> 
+      r' = Return\<^sub>e \<Longrightarrow> P) \<Longrightarrow> 
     P"
 proof (induction \<Sigma>\<^sub>c)
   case (SE\<^sub>c s\<^sub>c \<Delta>\<^sub>c e)
-  moreover then obtain \<C>'' where "stack_from_stack s\<^sub>c = (\<Delta>\<^sub>e, \<C>'') # s\<^sub>e \<and> 
-    encode e @ \<C>'' = PushLam\<^sub>e \<C>' # \<C>" by auto
+  moreover then obtain \<C>'' where "stack_from_stack s\<^sub>c = (\<Delta>\<^sub>e, \<C>'', r) # s\<^sub>e \<and> 
+    encode e @ \<C>'' = PushLam\<^sub>e \<C>' r' # \<C>" by auto
   moreover then obtain tt e' where "head_expr e = Lam\<^sub>d tt e' \<and> \<C>' = encode e' \<and> 
-    \<C> = tl (encode e) @ \<C>''" by (metis encode_to_pushlam)
+    \<C> = tl (encode e) @ \<C>'' \<and> r' = Return\<^sub>e" by (metis encode_to_pushlam)
   ultimately show ?case by auto
 qed auto
 
 lemma encode_state_to_apply [dest]: "
-  encode_state \<Sigma>\<^sub>c = S\<^sub>e (v # Lam\<^sub>e \<Delta>\<^sub>e' \<C>' # \<V>) ((\<Delta>\<^sub>e, Apply\<^sub>e # \<C>) # s\<^sub>e) \<Longrightarrow>
-    \<exists>s\<^sub>c c c'. \<Sigma>\<^sub>c = SC\<^sub>c (FApp2\<^sub>c c' # s\<^sub>c) c \<and> stack_from_stack s\<^sub>c = ((\<Delta>\<^sub>e, \<C>) # s\<^sub>e) \<and> 
-      v = encode_closure c \<and> Lam\<^sub>e \<Delta>\<^sub>e' \<C>' = encode_closure c' \<and> \<V> = vals_from_stack s\<^sub>c"
+  encode_state \<Sigma>\<^sub>c = S\<^sub>e (v # Lam\<^sub>e \<Delta>\<^sub>e' \<C>' r' # \<V>) ((\<Delta>\<^sub>e, Apply\<^sub>e # \<C>, r) # s\<^sub>e) \<Longrightarrow>
+    \<exists>s\<^sub>c c c'. \<Sigma>\<^sub>c = SC\<^sub>c (FApp2\<^sub>c c' # s\<^sub>c) c \<and> stack_from_stack s\<^sub>c = ((\<Delta>\<^sub>e, \<C>, r) # s\<^sub>e) \<and> 
+      v = encode_closure c \<and> Lam\<^sub>e \<Delta>\<^sub>e' \<C>' r' = encode_closure c' \<and> \<V> = vals_from_stack s\<^sub>c"
   by (induction \<Sigma>\<^sub>c) auto
 
-lemma encode_state_to_return [dest]: "encode_state \<Sigma>\<^sub>c = S\<^sub>e \<V> ((\<Delta>\<^sub>e, []) # s\<^sub>e) \<Longrightarrow> 
+lemma encode_state_to_return [dest]: "encode_state \<Sigma>\<^sub>c = S\<^sub>e \<V> ((\<Delta>\<^sub>e, [], Return\<^sub>e) # s\<^sub>e) \<Longrightarrow> 
   (\<exists>\<Delta>\<^sub>c s c. \<Sigma>\<^sub>c = SC\<^sub>c (FReturn\<^sub>c \<Delta>\<^sub>c # s) c \<and> s\<^sub>e = stack_from_stack s \<and>
     \<Delta>\<^sub>e = map encode_closure \<Delta>\<^sub>c \<and> \<V> = encode_closure c # vals_from_stack s)"
+  by (induction \<Sigma>\<^sub>c) auto
+
+lemma encode_state_to_jump [dest]: "encode_state \<Sigma>\<^sub>c = S\<^sub>e \<V> ((\<Delta>\<^sub>e, [], Jump\<^sub>e) # s\<^sub>e) \<Longrightarrow> False"
   by (induction \<Sigma>\<^sub>c) auto
 
 text \<open>And now, we can finally prove completeness.\<close>
@@ -319,8 +326,8 @@ text \<open>And now, we can finally prove completeness.\<close>
 theorem complete\<^sub>e [simp]: "encode_state \<Sigma>\<^sub>c \<leadsto>\<^sub>e \<Sigma>\<^sub>t' \<Longrightarrow> \<Sigma>\<^sub>c :\<^sub>c t \<Longrightarrow>
   \<exists>\<Sigma>\<^sub>c'. iter (\<leadsto>\<^sub>c) \<Sigma>\<^sub>c \<Sigma>\<^sub>c' \<and> \<Sigma>\<^sub>t' = encode_state \<Sigma>\<^sub>c'"
 proof (induction "encode_state \<Sigma>\<^sub>c" \<Sigma>\<^sub>t' rule: eval\<^sub>e.induct)
-  case (ev\<^sub>e_lookup \<Delta>\<^sub>e x v \<V> \<C> s\<^sub>e)
-  hence X: "encode_state \<Sigma>\<^sub>c = S\<^sub>e \<V> ((\<Delta>\<^sub>e, Lookup\<^sub>e x # \<C>) # s\<^sub>e)" by simp
+  case (ev\<^sub>e_lookup \<Delta>\<^sub>e x v \<V> \<C> r s\<^sub>e)
+  hence X: "encode_state \<Sigma>\<^sub>c = S\<^sub>e \<V> ((\<Delta>\<^sub>e, Lookup\<^sub>e x # \<C>, r) # s\<^sub>e)" by simp
   from X ev\<^sub>e_lookup(1, 3) show ?case
   proof (induction rule: encode_state_to_lookup)
     case (SE\<^sub>c s\<^sub>c \<Delta>\<^sub>c e \<C>')
@@ -341,8 +348,8 @@ proof (induction "encode_state \<Sigma>\<^sub>c" \<Sigma>\<^sub>t' rule: eval\<^
     with SC\<^sub>c C show ?case by auto
   qed
 next
-  case (ev\<^sub>e_pushcon \<V> \<Delta>\<^sub>e n \<C> s\<^sub>e)
-  hence X: "encode_state \<Sigma>\<^sub>c = S\<^sub>e \<V> ((\<Delta>\<^sub>e, PushCon\<^sub>e n # \<C>) # s\<^sub>e)" by simp
+  case (ev\<^sub>e_pushcon \<V> \<Delta>\<^sub>e n \<C> r s\<^sub>e)
+  hence X: "encode_state \<Sigma>\<^sub>c = S\<^sub>e \<V> ((\<Delta>\<^sub>e, PushCon\<^sub>e n # \<C>, r) # s\<^sub>e)" by simp
   from X ev\<^sub>e_pushcon(2) show ?case
   proof (induction rule: encode_state_to_pushcon)
     case (SE\<^sub>c s\<^sub>c \<Delta>\<^sub>c e \<C>')
@@ -362,18 +369,18 @@ next
     with SC\<^sub>c show ?case by auto
   qed
 next
-  case (ev\<^sub>e_pushlam \<V> \<Delta>\<^sub>e \<C>' \<C> s\<^sub>e)
-  hence X: "encode_state \<Sigma>\<^sub>c = S\<^sub>e \<V> ((\<Delta>\<^sub>e, PushLam\<^sub>e \<C>' # \<C>) # s\<^sub>e)" by simp
+  case (ev\<^sub>e_pushlam \<V> \<Delta>\<^sub>e \<C>' r' \<C> r s\<^sub>e)
+  hence X: "encode_state \<Sigma>\<^sub>c = S\<^sub>e \<V> ((\<Delta>\<^sub>e, PushLam\<^sub>e \<C>' r' # \<C>, r) # s\<^sub>e)" by simp
   from X ev\<^sub>e_pushlam(2) show ?case
   proof (induction rule: encode_state_to_pushlam)
     case (SE\<^sub>c s\<^sub>c \<Delta>\<^sub>c e tt e' \<C>'')
     moreover have "iter (\<leadsto>\<^sub>c) (SE\<^sub>c s\<^sub>c \<Delta>\<^sub>c e) (SE\<^sub>c (tail_expr \<Delta>\<^sub>c e @ s\<^sub>c) \<Delta>\<^sub>c (head_expr e))" by simp
     moreover have "SE\<^sub>c (tail_expr \<Delta>\<^sub>c e @ s\<^sub>c) \<Delta>\<^sub>c (Lam\<^sub>d tt e') \<leadsto>\<^sub>c 
       SC\<^sub>c (tail_expr \<Delta>\<^sub>c e @ s\<^sub>c) (Lam\<^sub>c tt \<Delta>\<^sub>c e')" by simp
-    ultimately have X: "iter (\<leadsto>\<^sub>c) (SE\<^sub>c s\<^sub>c \<Delta>\<^sub>c e) (SC\<^sub>c (tail_expr \<Delta>\<^sub>c e @ s\<^sub>c) (Lam\<^sub>c tt \<Delta>\<^sub>c e'))"
+    ultimately have E: "iter (\<leadsto>\<^sub>c) (SE\<^sub>c s\<^sub>c \<Delta>\<^sub>c e) (SC\<^sub>c (tail_expr \<Delta>\<^sub>c e @ s\<^sub>c) (Lam\<^sub>c tt \<Delta>\<^sub>c e'))"
       by (metis iter_step_after)
-    from SE\<^sub>c have "\<Delta>\<^sub>e = map encode_closure \<Delta>\<^sub>c" by fastforce
-    with SE\<^sub>c X show ?case by auto
+    from SE\<^sub>c have "\<Delta>\<^sub>e = map encode_closure \<Delta>\<^sub>c \<and> r' = Return\<^sub>e" by fastforce
+    with SE\<^sub>c E show ?case by auto
   next
     case (SC\<^sub>c s\<^sub>c c \<Delta>\<^sub>c e tt e' \<C>'')
     moreover have "iter (\<leadsto>\<^sub>c) (SE\<^sub>c (FApp2\<^sub>c c # s\<^sub>c) \<Delta>\<^sub>c e) 
@@ -381,17 +388,18 @@ next
     moreover have "SC\<^sub>c (FApp1\<^sub>c \<Delta>\<^sub>c e # s\<^sub>c) c \<leadsto>\<^sub>c SE\<^sub>c (FApp2\<^sub>c c # s\<^sub>c) \<Delta>\<^sub>c e" by simp
     moreover have "SE\<^sub>c (tail_expr \<Delta>\<^sub>c e @ FApp2\<^sub>c c # s\<^sub>c) \<Delta>\<^sub>c (Lam\<^sub>d tt e') \<leadsto>\<^sub>c 
       SC\<^sub>c (tail_expr \<Delta>\<^sub>c e @ FApp2\<^sub>c c # s\<^sub>c) (Lam\<^sub>c tt \<Delta>\<^sub>c e')" by simp
-    ultimately have X: "iter (\<leadsto>\<^sub>c) (SC\<^sub>c (FApp1\<^sub>c \<Delta>\<^sub>c e # s\<^sub>c) c) 
+    ultimately have E: "iter (\<leadsto>\<^sub>c) (SC\<^sub>c (FApp1\<^sub>c \<Delta>\<^sub>c e # s\<^sub>c) c) 
       (SC\<^sub>c (tail_expr \<Delta>\<^sub>c e @ FApp2\<^sub>c c # s\<^sub>c) (Lam\<^sub>c tt \<Delta>\<^sub>c e'))" 
         by (metis iter_step iter_step_after)
-    from SC\<^sub>c have "\<Delta>\<^sub>e = map encode_closure \<Delta>\<^sub>c" by fastforce
-    with SC\<^sub>c X show ?case by auto
+    from SC\<^sub>c have "\<Delta>\<^sub>e = map encode_closure \<Delta>\<^sub>c \<and> r' = Return\<^sub>e" by fastforce
+    with SC\<^sub>c E show ?case by auto
   qed
 next
-  case (ev\<^sub>e_apply v \<Delta>\<^sub>e' \<C>' \<V> \<Delta>\<^sub>e \<C> s\<^sub>e)
-  hence "encode_state \<Sigma>\<^sub>c = S\<^sub>e (v # Lam\<^sub>e \<Delta>\<^sub>e' \<C>' # \<V>) ((\<Delta>\<^sub>e, Apply\<^sub>e # \<C>) # s\<^sub>e)" by simp
-  then obtain s\<^sub>c c c' where "\<Sigma>\<^sub>c = SC\<^sub>c (FApp2\<^sub>c c' # s\<^sub>c) c \<and> stack_from_stack s\<^sub>c = ((\<Delta>\<^sub>e, \<C>) # s\<^sub>e) \<and> 
-    v = encode_closure c \<and> Lam\<^sub>e \<Delta>\<^sub>e' \<C>' = encode_closure c' \<and> \<V> = vals_from_stack s\<^sub>c" 
+  case (ev\<^sub>e_apply v \<Delta>\<^sub>e' \<C>' r' \<V> \<Delta>\<^sub>e \<C> r s\<^sub>e)
+  hence "encode_state \<Sigma>\<^sub>c = S\<^sub>e (v # Lam\<^sub>e \<Delta>\<^sub>e' \<C>' r' # \<V>) ((\<Delta>\<^sub>e, Apply\<^sub>e # \<C>, r) # s\<^sub>e)" by simp
+  then obtain s\<^sub>c c c' where "\<Sigma>\<^sub>c = SC\<^sub>c (FApp2\<^sub>c c' # s\<^sub>c) c \<and> 
+    stack_from_stack s\<^sub>c = ((\<Delta>\<^sub>e, \<C>, r) # s\<^sub>e) \<and> v = encode_closure c \<and> 
+    Lam\<^sub>e \<Delta>\<^sub>e' \<C>' r' = encode_closure c' \<and> \<V> = vals_from_stack s\<^sub>c" 
       by auto
   moreover then obtain t \<Delta>\<^sub>c e where "c' = Lam\<^sub>c t \<Delta>\<^sub>c e \<and> \<Delta>\<^sub>e' = map encode_closure \<Delta>\<^sub>c \<and> 
     \<C>' = encode e" by auto
@@ -402,7 +410,7 @@ next
   ultimately show ?case by auto
 next
   case (ev\<^sub>e_return \<V> \<Delta>\<^sub>e s\<^sub>e)
-  hence "encode_state \<Sigma>\<^sub>c = S\<^sub>e \<V> ((\<Delta>\<^sub>e, []) # s\<^sub>e)" by simp
+  hence "encode_state \<Sigma>\<^sub>c = S\<^sub>e \<V> ((\<Delta>\<^sub>e, [], Return\<^sub>e) # s\<^sub>e)" by simp
   then obtain \<Delta>\<^sub>c s\<^sub>c c where S: "\<Sigma>\<^sub>c = SC\<^sub>c (FReturn\<^sub>c \<Delta>\<^sub>c # s\<^sub>c) c \<and> s\<^sub>e = stack_from_stack s\<^sub>c \<and>
     \<Delta>\<^sub>e = map encode_closure \<Delta>\<^sub>c \<and> \<V> = encode_closure c # vals_from_stack s\<^sub>c" by auto
   have "SC\<^sub>c (FReturn\<^sub>c \<Delta>\<^sub>c # s\<^sub>c) c \<leadsto>\<^sub>c SC\<^sub>c s\<^sub>c c" by simp
